theories/prelude/fin_maps.v
@@ -118,7 +118,13 @@ Context `{FinMap K M}.
 
 (** ** Setoids *)
 Section setoid.
-  Context `{Equiv A} `{!Equivalence ((≡) : relation A)}.
+  Context `{Equiv A}.
+  
+  Lemma map_equiv_lookup_l (m1 m2 : M A) i x :
+    m1 ≡ m2 → m1 !! i = Some x → ∃ y, m2 !! i = Some y ∧ x ≡ y.
+  Proof. generalize (equiv_Some_inv_l (m1 !! i) (m2 !! i) x); naive_solver. Qed.
+
+  Context `{!Equivalence ((≡) : relation A)}.
   Global Instance map_equivalence : Equivalence ((≡) : relation (M A)).
   Proof.
     split.
@@ -173,9 +179,6 @@ Section setoid.
     split; [intros Hm; apply map_eq; intros i|by intros ->].
     by rewrite lookup_empty, <-equiv_None, Hm, lookup_empty.
   Qed.
-  Lemma map_equiv_lookup_l (m1 m2 : M A) i x :
-    m1 ≡ m2 → m1 !! i = Some x → ∃ y, m2 !! i = Some y ∧ x ≡ y.
-  Proof. generalize (equiv_Some_inv_l (m1 !! i) (m2 !! i) x); naive_solver. Qed.
   Global Instance map_fmap_proper `{Equiv B} (f : A → B) :
     Proper ((≡) ==> (≡)) f → Proper ((≡) ==> (≡)) (fmap (M:=M) f).
   Proof.
